wip

code/ecdsap256sha2/Hacl.Impl.P256.MM.Exponent.fst
@@ -18,14 +18,19 @@ open FStar.Mul
 
 open Lib.Loops
 
-open Hacl.Impl.ECDSA.MontgomeryMultiplication
+open Hacl.Impl.P256.MontgomeryMultiplication
+open Spec.P256.MontgomeryMultiplication
+
+open Hacl.Impl.P256.LowLevel
+open Hacl.Impl.P256.Arithmetics
 
 open Spec.P256.Definitions
-open Spec.P256
 open Spec.P256.Lemmas
 open Spec.P256.Ladder
+open Spec.P256
 
-#set-options "--z3rlimit 200 --max_fuel 0 --max_ifuel 0" 
+
+#set-options "--z3rlimit 200 --fuel 0 --ifuel 0" 
 
 [@ CInline]
 val cswap: bit:uint64{v bit <= 1} -> p:felem -> q:felem
@@ -36,7 +41,7 @@ val cswap: bit:uint64{v bit <= 1} -> p:felem -> q:felem
     (ensures  fun h0 _ h1 ->
       modifies (loc p |+| loc q) h0 h1 /\
 	(
-	  let (r0, r1) = Spec.ECDSA.conditional_swap bit (as_nat h0 p) (as_nat h0 q) in 
+	  let (r0, r1) = conditional_swap_exponent bit (as_nat h0 p) (as_nat h0 q) in 
 	  let pBefore = as_seq h0 p in let qBefore = as_seq h0 q in 
 	  let pAfter = as_seq h1 p in let qAfter = as_seq h1 q in 
 	  if uint_v bit = 0 then r0 == as_nat h0 p /\ r1 == as_nat h0 q else r0 == as_nat h0 q /\ r1 == as_nat h0 p) /\
@@ -71,9 +76,23 @@ let cswap bit p1 p2 =
   Lib.Sequence.eq_intro (as_seq h1 p2) (if v bit = 1 then as_seq h0 p1 else as_seq h0 p2)
 
 
+inline_for_extraction noextract 
+val upload_one_montg_form: b: felem -> Stack unit
+  (requires fun h -> live h b)
+  (ensures fun h0 _ h1 -> modifies (loc b) h0 h1 /\ as_nat h1 b == toDomain_ (1))
+
+let upload_one_montg_form b =
+  upd b (size 0) (u64 1);
+  upd b (size 1) (u64 18446744069414584320);
+  upd b (size 2) (u64 18446744073709551615);
+  upd b (size 3) (u64 4294967294);
+  
+  assert_norm (1 + 18446744069414584320 * pow2 64 + 18446744073709551615 * pow2 64 * pow2 64 + 4294967294 * pow2 64 * pow2 64 * pow2 64  == pow2 256 % prime256);
+  lemmaToDomain 1
+
 
 inline_for_extraction noextract
-val montgomery_ladder_exponent_step0: a: felem -> b: felem -> Stack unit
+val montgomery_ladder_power_step0: a: felem -> b: felem -> Stack unit
   (requires fun h -> live h a /\ live h b /\ as_nat h a < prime /\ as_nat h b < prime /\ disjoint a b )
   (ensures fun h0 _ h1 -> modifies (loc a |+| loc b) h0 h1 /\ as_nat h1 a < prime /\ as_nat h1 b < prime /\
     (
@@ -83,9 +102,167 @@ val montgomery_ladder_exponent_step0: a: felem -> b: felem -> Stack unit
     )
 )
 
-let montgomery_ladder_exponent_step0 a b = 
+let montgomery_ladder_power_step0 a b = 
     let h0 = ST.get() in 
-  montgomery_multiplication_ecdsa_module a b b;
-    lemmaToDomainFromDomain (fromDomain_ (as_nat h0 a) * fromDomain_ (as_nat h0 b) % prime);
-  montgomery_multiplication_ecdsa_module a a a ;
-    lemmaToDomainFromDomain (fromDomain_ (as_nat h0 a) * fromDomain_ (as_nat h0 a) % prime)
+    montgomery_multiplication_buffer a b b;
+    lemmaToDomainAndBackIsTheSame (fromDomain_ (as_nat h0 a) * fromDomain_ (as_nat h0 b) % prime);
+  montgomery_multiplication_buffer a a a ;
+    lemmaToDomainAndBackIsTheSame (fromDomain_ (as_nat h0 a) * fromDomain_ (as_nat h0 a) % prime)
+
+
+inline_for_extraction noextract
+val montgomery_ladder_power_step: a: felem -> b: felem -> scalar: lbuffer uint8 (size 32) ->   i:size_t{v i < 256} ->  Stack unit
+  (requires fun h -> live h a  /\ live h b /\ live h scalar /\ as_nat h a < prime /\ as_nat h b < prime /\ disjoint a b)
+  (ensures fun h0 _ h1 -> modifies (loc a |+| loc b) h0 h1  /\
+    (
+      let a_ = fromDomain_ (as_nat h0 a) in 
+      let b_ = fromDomain_ (as_nat h0 b) in 
+      let (r0D, r1D) = _exp_step (as_seq h0 scalar) (uint_v i) (a_, b_) in 
+      r0D == fromDomain_ (as_nat h1 a) /\ r1D == fromDomain_ (as_nat h1 b) /\ 
+      as_nat h1 a < prime /\ as_nat h1 b < prime 
+    ) 
+  )  
+
+let montgomery_ladder_power_step a b scalar i = 
+    let h0 = ST.get() in 
+  let bit0 = (size 255) -. i in 
+  let bit = scalar_bit scalar bit0 in 
+  cswap bit a b;
+  montgomery_ladder_power_step0 a b;
+  cswap bit a b;
+    admit();
+    lemma_swaped_steps (fromDomain_ (as_nat h0 a)) (fromDomain_ (as_nat h0 b))
+
+
+inline_for_extraction noextract 
+val _montgomery_ladder_power: a: felem -> b: felem -> scalar: ilbuffer uint8 (size 32) -> Stack unit
+  (requires fun h -> live h a /\ live h b /\ live h scalar /\ as_nat h a < prime /\ 
+    as_nat h b < prime /\ disjoint a b /\disjoint a scalar /\ disjoint b scalar)
+  (ensures fun h0 _ h1 -> modifies (loc a |+| loc b) h0 h1 /\ 
+    (
+      let a_ = fromDomain_ (as_nat h0 a) in 
+      let b_ = fromDomain_ (as_nat h0 b) in 
+      let (r0D, r1D) = _exponent_spec (as_seq h0 scalar) (a_, b_) in 
+      r0D == fromDomain_ (as_nat h1 a) /\ r1D == fromDomain_ (as_nat h1 b) /\
+      as_nat h1 a < prime /\ as_nat h1 b < prime )
+  )
+
+  
+let _montgomery_ladder_power a b scalar = 
+  let h0 = ST.get() in 
+  [@inline_let]
+  let spec_exp h0  = _exp_step (as_seq h0 scalar) in 
+  [@inline_let]
+  let acc (h: mem) : GTot (tuple2 nat_prime nat_prime) = (fromDomain_ (as_nat h a), fromDomain_ (as_nat h b)) in 
+  Lib.LoopCombinators.eq_repeati0 256 (spec_exp h0) (acc h0);
+  [@inline_let]
+  let inv h (i: nat {i <= 256}) = 
+    live h a /\ live h b /\ live h scalar /\ modifies (loc a |+| loc b) h0 h /\ as_nat h a < prime /\ as_nat h b < prime /\
+    acc h == Lib.LoopCombinators.repeati i (spec_exp h0) (acc h0) in 
+  for 0ul 256ul inv (
+    fun i -> 
+	  montgomery_ladder_power_step a b scalar i;
+	  Lib.LoopCombinators.unfold_repeati 256 (spec_exp h0) (acc h0) (uint_v i))
+
+
+val montgomery_ladder_power: a: felem -> scalar: ilbuffer uint8 (size 32) ->  Stack unit 
+  (requires fun h -> live h a /\ as_nat h a < prime)
+  (ensures fun h0 _ h1 -> modifies (loc a) h0 h1
+)
+
+
+let montgomery_ladder_power r scalar = 
+  push_frame(); 
+    let p = create (size 4) (u64 0) in 
+    upload_one_montg_form p; 
+    recall_contents prime256_buffer (Lib.Sequence.of_list p256_prime_list);
+    _montgomery_ladder_power p r scalar;
+      lemmaToDomainAndBackIsTheSame 1;
+    copy r p;
+  pop_frame()  
+
+
+(* sqPower =  (prime + 1) // 4 *)
+val uploadSQpower: a: felem -> Stack unit 
+  (requires fun h -> live h a)
+  (ensures fun h0 _ h1 -> modifies (loc a) h0 h1 /\ as_nat h1 a == 28948022302589062190674361737351893382521535853822578548883407827216774463488)
+
+let uploadSQpower a = 
+  upd a (size 0) (u64 0);
+  upd a (size 1) (u64 1073741824);
+  upd a (size 2) (u64 4611686018427387904);
+  upd a (size 3) (u64 4611686017353646080)
+
+
+val square_root: a: felem -> Stack unit 
+  (requires fun h -> True)
+  (ensures fun h0 _ h1 -> True)
+
+let square_root a  = 
+  push_frame();
+    let sqPower = create (size 4) (u64 0) in 
+    uploadSQpower sqPower;
+    montgomery_ladder_power a sqPower;
+  pop_frame()
+
+
+
+val uploadA: a: felem -> Stack unit
+  (requires fun h -> live h a)
+  (ensures fun h0 _ h1 -> modifies (loc a) h0 h1 /\ as_nat h1 a == aCoordinateP256 % prime256)
+
+let uploadA a = 
+  upd a (size 0) (u64 18446744073709551612);
+  upd a (size 1) (u64 4294967295);
+  upd a (size 2) (u64 0);
+  upd a (size 3) (u64 18446744069414584321);
+  assert_norm(18446744073709551612 + 4294967295 * pow2 64 + 18446744069414584321 * pow2 64 * pow2 64 * pow2 64 = aCoordinateP256 % prime256)
+  
+
+val uploadB: b: felem -> Stack unit 
+  (requires fun h -> live h b)
+  (ensures fun h0 _ h1 -> modifies (loc b) h0 h1 /\ as_nat h1 b == bCoordinateP256)
+
+let uploadB b = 
+  upd b (size 0) (u64 4309448131093880907);
+  upd b (size 1) (u64 7285987128567378166);
+  upd b (size 2) (u64 12964664127075681980);
+  upd b (size 3) (u64 6540974713487397863);
+  assert_norm (4309448131093880907 + 7285987128567378166 * pow2 64 + 12964664127075681980 * pow2 64 * pow2 64 + 6540974713487397863 * pow2 64 * pow2 64 * pow2 64 == 41058363725152142129326129780047268409114441015993725554835256314039467401291)
+
+
+
+val computeYFromX: x: felem ->  result: felem -> sign: uint64 -> Stack unit 
+  (requires fun h -> live h x /\ live h result /\ as_nat h x < prime)
+  (ensures fun h0 _ h1 -> True)
+
+
+let computeYFromX x result sign = 
+  push_frame();
+    let aCoordinateBuffer = create (size 4) (u64 0) in 
+    let bCoordinateBuffer = create (size 4) (u64 0) in 
+   
+    uploadA aCoordinateBuffer;
+    uploadB bCoordinateBuffer;
+
+    montgomery_multiplication_buffer aCoordinateBuffer x aCoordinateBuffer;
+
+    cube x result;
+    p256_add result aCoordinateBuffer result;
+    p256_add result bCoordinateBuffer result;
+
+    uploadZeroImpl aCoordinateBuffer;
+    p256_sub aCoordinateBuffer result bCoordinateBuffer;
+
+    cmovznz4 sign bCoordinateBuffer result result;
+
+    square_root result;
+
+
+    admit();
+    
+
+
+ pop_frame()   
+    
+    
